Unbind in Coq, thanks to tchajed

test/highorder/unbind.v
@@ -1,42 +1,146 @@
 Require Export Coq.Lists.List.
+Require Eqdep.
+Require Import RelationClasses.
 Import ListNotations.
 
 Set Implicit Arguments.
 
+Ltac sigT_eq :=
+  match goal with
+  | [ H: existT ?P ?a _ = existT ?P ?a _ |- _ ] =>
+    apply Eqdep.EqdepTheory.inj_pair2 in H; subst
+  end.
+
+Ltac inv H := inversion H; subst; clear H; repeat sigT_eq.
+
+
+Inductive opT : Type -> Type :=
+| print : nat -> opT unit
+| getline : opT nat.
+
 Inductive proc: Type -> Type :=
 | ret: forall T, T -> proc T
 | bind: forall T T', proc T -> (T -> proc T') -> proc T'
-| print: nat -> proc unit.
+| runlist: forall T, list (opT T) -> proc unit
+| prim: forall T, opT T -> proc T.
+Definition event := sigT (fun T => opT T).
 
-Fixpoint f(a: nat) :=
-  match a with
-    | 0 => ret tt
-    | S n => bind (print a) (fun _ => f n)
-  end.
+(*Definition event := {T & opT T}. *)
+Definition ev T (op:opT T) : event :=
+  existT _ _ op.
 
-Compute f 2.
+Inductive step : forall T, opT T -> T -> Prop :=
+| step_print : forall n,
+    step (print n) tt
+| step_getline : forall n,
+    step getline n
+.
 
-Definition foo := bind (print 2) 
-                       (fun _ => bind (print 1) 
+Definition trace := list event.
+
+Inductive step_list : forall T, list (opT T) -> trace -> Prop :=
+| step_list_nil : forall T, step_list (@nil (opT T)) nil
+| step_list_cons : forall T (op:opT T) (l: list (opT T)) r tr,
+    step op r ->
+    step_list l tr ->
+    step_list (op::l) (ev op::tr)
+.
+
+(* [exec p r tr] means that p runs and returns r, while printing tr *)
+Inductive exec : forall T, proc T -> T -> trace -> Prop :=
+| exec_prim : forall T (op:opT T) r,
+    step op r ->
+    exec (prim op) r [ev op]
+| exec_ret : forall T (v:T),
+    exec (ret v) v []
+| exec_bind : forall T T' (p: proc T) (p': T -> proc T') r tr r' tr',
+    exec p r tr ->
+    exec (p' r) r' tr' ->
+    exec (bind p p') r' (tr ++ tr')
+| exec_runlist : forall T (ops: list (opT T)) tr,
+    step_list ops tr ->
+    exec (runlist ops) tt tr
+.
+
+Hint Constructors exec.
+
+Definition equiv T (p p':proc T) : Prop :=
+  forall r tr, exec p r tr <-> exec p' r tr.
+
+Definition Print a := prim (print a).
+
+Hint Constructors step_list.
+
+Theorem ret_getlist : forall T,
+    equiv (ret tt) (@runlist T []).
+Proof.
+  intros.
+  unfold equiv; split; intros.
+  destruct r.
+  inv H; eauto.
+  inv H.
+  inv H3; eauto.
+Qed.
+
+Theorem bind_getlist : forall T (op:opT T) l,
+    equiv (bind (prim op) (fun _ => runlist l))
+          (runlist (op::l)).
+Admitted.
+
+Theorem bind_congruence : forall T (p p': proc T) T' (rx rx': T -> proc T'),
+    equiv p p' ->
+    (forall x, equiv (rx x) (rx' x)) ->
+    equiv (bind p rx) (bind p' rx').
+Admitted.
+
+Instance equiv_Equivalence T : Equivalence (equiv (T:=T)).
+constructor; hnf; intros.
+firstorder.
+firstorder.
+unfold equiv, iff in *; intros.
+specialize (H r tr).
+specialize (H0 r tr).
+intuition auto.
+Defined.
+
+(** Small example *)
+Definition foo := bind (Print 2)
+                       (fun _ => bind (Print 1)
                                    (fun _ => ret tt)).
 
-Definition bar := bind (print 2) 
-                       (fun _ => ret tt).
+Definition foo' := runlist [print 2; print 1].
 
+Definition foo_opt : {foo_opt | equiv foo foo_opt}.
+  unfold foo, Print.
+  eexists.
 
-Fixpoint unbind_no_f {T}(b: proc T) :=
-  match b with
-    | bind a f => (unbind_no_f a) (** How to match on lambda f? *)
-    | ret _ => []
-    | print n => [print n]
+  etransitivity.
+  eapply bind_congruence; intros.
+  reflexivity.
+
+  etransitivity.
+  eapply bind_congruence; intros.
+  reflexivity.
+  eapply ret_getlist.
+
+  repeat match goal with
+  | |- equiv (bind (prim ?op) ?rx) _ =>
+    match eval simpl in (rx tt) with
+    | runlist ?l => eapply (bind_getlist op l)
+    end
   end.
 
-Compute unbind_no_f(foo).
-
-Fixpoint unbind {T}(b: proc T) :=
-  match b with
-    | bind a (fun _ => f) => (unbind a) ++ (unbind f) (** How to match on lambda f? *)
-    | ret _ => []
-    | print n => [print n]
+  match goal with
+  | |- equiv (bind (prim ?op) ?rx) _ =>
+    match eval simpl in (rx tt) with
+    | runlist ?l => eapply (bind_getlist op l)
+    end
   end.
+Defined.
 
+Definition foo_p := ltac:(let x := eval simpl in (proj1_sig foo_opt) in
+                              match x with
+                              | runlist ?l => exact l
+                              end).
+
+Print foo_p.
